\documentclass{article}
\usepackage{epsfig}
\pagestyle{empty}
\begin{document}
$ n\log n $
\pagebreak

$n \log n$
\pagebreak

$n\log n$
\pagebreak

$\sin(x)$
\pagebreak

$\cos(x)$
\pagebreak

$a\sin(x) + b\cos(x)$
\pagebreak

$a\sin^2(x) + b\sin(x)\cos(x) + c\cos^2(x)$
\pagebreak

$ d_{cut} $
\pagebreak

$ N_{jet} $
\pagebreak

$ p_T $
\pagebreak

$ N_{jets} $
\pagebreak

$p_T$
\pagebreak

$\eta$
\pagebreak

$\phi$
\pagebreak

$ \eta $
\pagebreak

$ \varphi $
\pagebreak

$ \vareta $
\pagebreak

$ \phi $
\pagebreak

$r$
\pagebreak

$\lambda$
\pagebreak

$\theta$
\pagebreak

$x$
\pagebreak

$y$
\pagebreak

$z$
\pagebreak

$\sqrt(x^2+y^2+z^2)$
\pagebreak

$ (\eta,\phi) $
\pagebreak

$ (0.,0., 0., 0.) $
\pagebreak

$ ( \eta, \phi ) $
\pagebreak

$ y = \eta $
\pagebreak

$ m = 0 $
\pagebreak

$ p_{\mathrm{T}} $
\pagebreak

$ y $
\pagebreak

$ E $
\pagebreak

$ e \to p_{\mathrm{T}} $
\pagebreak

$ m_{\mathrm{tower}} = 0 $
\pagebreak

$ [-\pi,\pi] $
\pagebreak

\[ \textrm{xSlope} = \frac{x_{\textrm{end}} - x_{\textrm{begin}}} {z_{\textrm{end}} - z_{\textrm{begin}}} \]
\pagebreak

\[ \textrm{ySlope} = \frac{y_{\textrm{end}} - y_{\textrm{begin}}} {z_{\textrm{end}} - z_{\textrm{begin}}} \]
\pagebreak

$\chi^2$
\pagebreak

$ w_{x} $
\pagebreak

$ w_{y} $
\pagebreak

$ w_{\rm T} $
\pagebreak

$ p_{x}^{\rm miss} $
\pagebreak

$ p_{y}^{\rm miss} $
\pagebreak

$ E_{\rm T}^{\rm miss} = \sqrt{(p_{x}^{\rm miss})^{2} + (p_{y}^{\rm miss})^{2}} $
\pagebreak

$ \phi(E_{\rm T}^{\rm miss}) $
\pagebreak

$ \Sigma E_{\rm T} $
\pagebreak

$ p_{x} $
\pagebreak

$ p_{y} $
\pagebreak

$(p_{x},p_{y},\Sigma E_{\rmT}) $
\pagebreak

\begin{eqnarray*} p_{x}^{\rm miss} & = & - \sum p_{x} \\ p_{y}^{\rm miss} & = & - \sum p_{y} \\ \Sigma E_{\rm T} & = & \sum p_{\rm T}. \end{eqnarray*}
\pagebreak

$ p_{x,y} $
\pagebreak

$ p_{\rm T} $
\pagebreak

$ (p_{x},p_{y},\Sigma E_{\rm T}) $
\pagebreak

$ p_{\rm T} = \sqrt{ p_{x}^{2} + p_{y}^{2} } $
\pagebreak

$ E_{\rm T}^{\rm miss} $
\pagebreak

\begin{eqnarray*} p_{x}^{\rm miss} & \to & p_{x}^{\rm miss} - p_{x}^{\rm particle} \\ p_{y}^{\rm miss} & \to & p_{y}^{\rm miss} - p_{y}^{\rm particle} \\ \Sigma E_{\rm T} & \to & \Sigma E_{\rm T} + p_{\rm T}^{\rm particle} . \end{eqnarray*}
\pagebreak

$ p_{x}^{\rm particle} $
\pagebreak

$ p_{y}^{\rm particle} $
\pagebreak

$ p_{\rm T}^{\rm particle} $
\pagebreak

\begin{eqnarray*} p_{x}^{\rm miss} & \to & p_{x}^{\rm miss} - f \cdot p_{x}^{\rm particle} \\ p_{y}^{\rm miss} & \to & p_{y}^{\rm miss} - f \cdot p_{y}^{\rm particle} \\ \Sigma E_{\rm T} & \to & \Sigma E_{\rm T} + f \cdot p_{\rm T}^{\rm particle} . \end{eqnarray*}
\pagebreak

$ f $
\pagebreak

\begin{eqnarray*} p_{x}^{\rm miss} & \to & p_{x}^{\rm miss} + p_{x}^{\rm particle} \\ p_{y}^{\rm miss} & \to & p_{y}^{\rm miss} + p_{y}^{\rm particle} \\ \Sigma E_{\rm T} & \to & \Sigma E_{\rm T} - p_{\rm T}^{\rm particle} . \end{eqnarray*}
\pagebreak

\begin{eqnarray*} p_{x}^{\rm miss} & \to & p_{x}^{\rm miss} + p_{x}^{{\rm miss}\prime} \\ p_{y}^{\rm miss} & \to & p_{y}^{\rm miss} + p_{y}^{{\rm miss}\prime} \\ \Sigma E_{\rm T} & \to & \Sigma E_{\rm T} + \Sigma E_{\rm miss}^{\prime} . \end{eqnarray*}
\pagebreak

$ (p_{x}^{\rm miss},p_{y}^{\rm miss},\Sigma E_{\rm T}) $
\pagebreak

$ (p_{x}^{{\rm miss}\prime},p_{y}^{{\rm miss}\prime},\Sigma E_{\rm T}^{\prime}) $
\pagebreak

\begin{eqnarray*} p_{x}^{\rm miss} & \to & p_{x}^{\rm miss} - p_{x}^{{\rm miss}\prime} \\ p_{y}^{\rm miss} & \to & p_{y}^{\rm miss} - p_{y}^{{\rm miss}\prime} \\ \Sigma E_{\rm T} & \to & \Sigma E_{\rm T} - \Sigma E_{\rm miss}^{\prime} . \end{eqnarray*}
\pagebreak

\begin{eqnarray*} p_{x}^{\rm miss} & \to & f \cdot p_{x}^{\rm miss} \\ p_{y}^{\rm miss} & \to & f \cdot p_{y}^{\rm miss} \\ \Sigma E_{\rm T} & \to & f \cdot \Sigma E_{\rm T} \end{eqnarray*}
\pagebreak

\begin{eqnarray*} p_{x}^{\rm miss} & \to & p_{x}^{\rm miss} / f \\ p_{y}^{\rm miss} & \to & p_{y}^{\rm miss} / f \\ \Sigma E_{\rm T} & \to & \Sigma E_{\rm T} / f \end{eqnarray*}
\pagebreak

$ f = 0 $
\pagebreak

$ p_{x} = 0 $
\pagebreak

$ p_{y} = 0 $
\pagebreak

$ \Sigma E_{\rm T} = 0 $
\pagebreak

$ P_{x} $
\pagebreak

$ P_{y} $
\pagebreak

$ P_{z} $
\pagebreak

$ i \in \{ 0 \ldots N_{\rm objects} - 1 \} $
\pagebreak

$ N_{\rm objects} $
\pagebreak

$ i = 0 \ldots N_{\rm objects} - 1 $
\pagebreak

$ c_{x} $
\pagebreak

$ c_{y} $
\pagebreak

$ c_{z} $
\pagebreak

$ c_{T} $
\pagebreak

$ c_{e} $
\pagebreak

$ p_{x,{\rm miss}} = -\sum p_{x} $
\pagebreak

$ p_{y,{\rm miss}} = -\sum p_{x} $
\pagebreak

$ \sigma E_{\rm T} = \sum p_{\rm T} $
\pagebreak

$ \Delta = | x - y | $
\pagebreak

$ ( x, y ) $
\pagebreak

$ \Delta_{\rm min} $
\pagebreak

$ \Delta < \Delta_{\rm min} $
\pagebreak

$ x $
\pagebreak

$ f = x/y $
\pagebreak

\begin{eqnarray*} f & = & \left\{ \begin{array}{2} x/y & y \neq 0 \\ 0 & y = 0 \end{array} \right. \end{eqnarray*}
\pagebreak

$ (w_{x},w_{y},w_{\rm T}) $
\pagebreak

$ (p_{x},p_{y},p_{\rm T}) $
\pagebreak

$ (p_{x}^{\rm miss}, p_{y}^{\rm miss}, \Sigma E_{\rm T}) $
\pagebreak

$ (w_{x} p_{x}, w_{y} p_{y}, w_{\rm T} p_{\rm T}) $
\pagebreak

$ i = 1 \ldots N $
\pagebreak

\begin{eqnarray} p_{x}^{\rm miss} & = & - \sum_{i = 1}^{N} w_{x,i} p_{x,i} \ \ p_{y}^{\rm miss} & = & - \sum_{i = 1}^{N} w_{y,i} p_{y,i} \ \ \Sigma E_{\rm T} & = & \sum_{i = 1}^{N} w_{{\rm T},i} p_{{\rm T},i} \end{eqnarray}
\pagebreak

$ (w_{x} = 1, w_{y} = 1, w_{\rm T} = 1) $
\pagebreak

\[ \mathcal{W} + \mathcal{W}^{\prime} = \left(\begin{array}{c} w_{x} + w_{x}^{\prime} \\ w_{y} + w_{y}^{\prime} \\ w_{\rm T} + w_{\rm T}^{\prime} \end{array} \right) \]
\pagebreak

$ \mathcal{W}, \mathcal{W}^{\prime} $
\pagebreak

$ \mathcal{W} $
\pagebreak

\[ \mathcal{W} - \mathcal{W}^{\prime} = \left(\begin{array}{c} w_{x} - w_{x}^{\prime} \\ w_{y} - w_{y}^{\prime} \\ w_{\rm T} - w_{\rm T}^{\prime} \end{array} \right) \]
\pagebreak

$ \mathcal{W}^{\prime} $
\pagebreak

\[ s \times \mathcal{W} = \left( \begin{array}{c} w_{x} \times w_{x}^{\prime} \\ w_{y} \times w_{y}^{\prime} \\ w_{\rm T} \times = w_{\rm T}^{\prime} \end{array} \right) \]
\pagebreak

$ \mathcal{W}^{\prime} = (w_{x}^{\prime},w_{y}^{\prime},w_{\rm T}^{\prime}) $
\pagebreak

$ \mathcal{W}*{\prime} $
\pagebreak

\[ \mathcal{W} / s = \left( \begin{array}{c} w_{x} / w_{x}^{\prime} \\ w_{y} / w_{y}^{\prime} \\ w_{\rm T} / w_{\rm T}^{\prime} / s \end{array} \right) \]
\pagebreak

\[ s \times \mathcal{W} = \left( \begin{array}{c} s \times w_{x} \\ s \times w_{y} \\ s \times w_{\rm T} \end{array} \right) \]
\pagebreak

$ s $
\pagebreak

\[ \mathcal{W} / s = \left( \begin{array}{c} w_{x} / s \\ w_{y} / s \\ w_{\rm T} / s \end{array} \right) \]
\pagebreak

$ s = 0 $
\pagebreak

$ \chi^2 $
\pagebreak

$e_T$
\pagebreak

$( d_0, z_0, \phi, \theta, q/p )$
\pagebreak

$d_0$
\pagebreak

$z_0$
\pagebreak

$-\pi$
\pagebreak

$+\pi$
\pagebreak

$\pi$
\pagebreak

$q/p$
\pagebreak

$\left(\begin{array}{c}d_0\\z_0\\\phi_0\\\theta\\q/p\end{array}\right)$
\pagebreak

$\left(\begin{array}{c}d_0\\z_0\\\phi_0\\\theta\\1/p\\\end{array}\right)$
\pagebreak

$\left(\begin{array}{c}d_0\\z_0\\\phi_0\\\theta\\q/p\\\end{array}\right)$
\pagebreak

$(x,y,z,p_x,p_y,p_z)$
\pagebreak

$\mathrm{v}(a1,a2,a3 ... a_{15})$
\pagebreak

$\left(\begin{array}{ccccc} a_1 & a_2 & a_4 & a_7 & a_{11} \\ a_2 & a_3 & a_5 & a_8 & a_{12} \\ a_4 & a_5 & a_6 & a_9 & a_{13} \\ a_7 & a_8 & a_9 & a_{10} & a_{14} \\ a_{11} & a_{12} & a_{13} & a_{14} & a_{15} \end{array}\right)$
\pagebreak

$E_T$
\pagebreak

$E_T / p_T$
\pagebreak

$\alpha$
\pagebreak

$\beta$
\pagebreak

$E^2-p^2$
\pagebreak

$|\eta|$
\pagebreak

$|y|$
\pagebreak

\end{document}
